wip

Veir/Data/Refinement.lean
@@ -25,7 +25,7 @@ def IntIsRefinedByReg [DecidableEq Prop] (i : Veir.Data.LLVM.Int 64) (r : Veir.D
   In particular, any concrete `i'` refines a poison `i`, but a poison `i'` does *not* refine
   any `i`.
 -/
-def isRefinedBy [DecidableEq Prop] (i i' : Veir.Data.LLVM.Int 64)  : Prop :=
+def IntIsRefinedByInt [DecidableEq Prop] (i i' : Veir.Data.LLVM.Int 64) : Prop :=
   match i with
   | .val v =>
     match i' with
