Veir/Passes/InstructionSelection/Proofs.lean
@@ -22,6 +22,10 @@ theorem constant:
     IntIsRefinedByReg (Data.LLVM.Int.constant 64 v) (Data.RISCV.li (BitVec.ofInt 64 v)) := by
   simp [IntIsRefinedByReg, Data.LLVM.Int.constant, Data.RISCV.li]
 
+theorem constant':
+    IntIsRefinedByInt (Data.LLVM.Int.constant 64 v) (RISCV.Reg.toInt (Data.RISCV.li (BitVec.ofInt 64 v)) 64) := by
+  simp [IntIsRefinedByInt, Data.LLVM.Int.constant, Data.RISCV.li, RISCV.Reg.toInt]
+
 /--
   Prove the correctness of the `add` lowering pattern.
 -/
@@ -32,6 +36,21 @@ theorem add:
   split
   · split
     · split
+      <;> bv_decide
+    · split
+      · bv_decide
+      · simp only [Id.run, Data.LLVM.Int.val.injEq] at *
+        bv_decide
+  · bv_decide
+
+theorem add':
+    IntIsRefinedByInt (Data.LLVM.Int.add x y) (RISCV.Reg.toInt (Data.RISCV.add (LLVM.Int.toReg x) (LLVM.Int.toReg y)) 64) := by
+  simp only [IntIsRefinedByInt, Data.LLVM.Int.add, Bool.false_eq_true, false_and, ↓reduceIte,
+    pure_bind, Data.RISCV.add, LLVM.Int.toReg, BitVec.truncate_eq_setWidth, BitVec.setWidth_eq]xw
+  split
+  · split
+    · bv_decide
+      split
       <;> bv_decide
     · split
       · bv_decide
